Beta-eq relation

formal/SkLean/Eval.lean
@@ -6,11 +6,11 @@ def eval_once : Ast.Expr → Option Ast.Expr
   | SKM[((((K _α) _β) x) _y)] => pure x
   | SKM[((((((S _α) _β) _γ) x) y) z)] => pure SKM[((x z) (y z))]
   | SKM[(((M K) α) β)]     => pure SKM[(α ~> (β ~> α))]
-  | SKM[((((M S) α) β) γ)] => do
-    let lhs' := (eval_once SKM[(α γ)]).getD SKM[(α γ)]
-    let rhs' := (eval_once SKM[(β γ)]).getD SKM[(β γ)]
-
-    pure SKM[(lhs' rhs')]
+  | SKM[((((M S) α) β) γ)] => pure SKM[(α ~> β ~> γ ~> ((α γ) (β γ)))]
+  | SKM[((M M) K)] => pure SKM[Prp]
+  | SKM[((M M) S)] => pure SKM[Prp]
+  | SKM[((M M) M)] => pure SKM[Prp]
+  | SKM[((M M) #~>)] => pure SKM[Prp]
   | SKM[(M (lhs rhs))] => pure SKM[((M lhs) rhs)]
   | SKM[(M Ty n)] => SKM[Ty n.succ]
   | SKM[(M Prp)] => SKM[Ty 0]
@@ -19,4 +19,12 @@ def eval_once : Ast.Expr → Option Ast.Expr
   | SKM[(lhs rhs)] => do SKM[((#(← eval_once lhs)) rhs)]
   | _ => .none
 
+def eval_n : ℕ → Ast.Expr → Option Ast.Expr
+  | 0, _ => .none
+  | n + 1, e => do
+    let e' ← eval_once e
+    eval_n n e'
+
 end Expr
+
+def BetaEq := Relation.ReflTransGen (λ x y => Expr.eval_once x = .some y ∨ Expr.eval_once y = .some x)
