formal/SkLean/Judgment.lean
@@ -1,0 +1,42 @@
+import SkLean.Ast3
+import SkLean.Eval
+
+inductive IsComb : Ast.Expr → Prop
+  | k   : IsComb SKM[K]
+  | s   : IsComb SKM[S]
+  | m   : IsComb SKM[M]
+  | arr : IsComb SKM[#~>]
+
+inductive HasType : Ast.Expr → Ast.Expr → Prop
+  | comb : IsComb e
+    → HasType e SKM[(M e)]
+  | k₁   : HasType α t_α
+    → HasType SKM[(K α)] SKM[((M K) α)]
+  | k    : HasType α t_α
+    → HasType β t_β
+    → HasType SKM[((K α) β)] SKM[(α ~> β ~> α)]
+  | s₁   : HasType α t_α
+    → HasType SKM[(S α)] SKM[((M S) α)]
+  | s₂   : HasType α t_α
+    → HasType β t_β
+    → HasType SKM[((S α) β)] SKM[(((M S) α) β)]
+  | s    : HasType α t_α
+    → HasType β t_β
+    → HasType γ t_γ
+    → HasType SKM[(((S α) β) γ)] SKM[(α ~> β ~> γ ~> ((α γ) (β γ)))]
+  | m_m  : IsComb e
+    → HasType SKM[(M e)] SKM[Prp]
+  | prp  : HasType SKM[Prp] SKM[Ty 0]
+  | ty   : HasType SKM[Ty n] SKM[Ty n.succ]
+  | arr  : HasType SKM[t_in ~> t_out] SKM[Ty 0]
+  -- Non-dependent
+  | call : HasType lhs SKM[t_in ~> t_out]
+    → HasType rhs t_in
+    → HasType SKM[(lhs rhs)] t_out
+
+namespace HasType
+
+theorem preservation (h : HasType e t) (h : Expr.eval_once e = .some e') : HasType e' t := by
+  sorry
+
+end HasType
